\documentclass[20pt,a4paper]{extarticle} %big fontsize
\usepackage[margin=0.7in]{geometry}
\usepackage{amsmath,amsthm,amssymb}
\usepackage{enumitem,amsfonts,extarrows,xcolor}

\theoremstyle{definition}
\newtheorem{example}{Example}[section]

\theoremstyle{definition}
\newtheorem{definition}{Definiton}[section]

\begin{document}
\paragraph{Final Exam}

\section*{Question 1}
Given that $c \in (a,b)$,with \\(a) $f \in R[a,c]$ and \\(b) $f \in R[b,c]$\\
Need that $f \in R[a,b]$
\begin{proof}
	Need to show that,
	\[ \forall \epsilon > 0, \exists P \in \mathbb{P}([a,b]) : U(P,f) - L(P,f) < \epsilon \]

	Fix any $\epsilon>0$.\\
	By (a), have that
	\[ \exists P \in \mathbb{P}([a,c]) : U(P,f) - L(P,f) < \frac{\epsilon}{2} \]
	By (b), have that
	\[ \exists Q \in \mathbb{P}([c,b]) : U(Q,f) - L(Q,f) < \frac{\epsilon}{2}\]
	Consider
	\[ U(P,f)+U(Q,f)= \sum_{i=1}^{p}M_i \delta t_i + \sum_{i=1}^{q}M'_i \delta t'_i   \]
	where $M_i$ and $t_i$ correspond to P, while where $M'_i$ and $t'_i$ correspond to Q.
	\newpage
	Taking $S:= P \cup Q$ so that $S \in \mathbb{P}([a,b]) $,\\
	giving S=$\{a<t_1<t_2<...<c<t'_1<t'_2<...<b\}$

	where $t_i \in P$ and $t'_i \in Q$, so that,\\
	\begin{align*}
		U(S,f)&= \sum_{i=1}^{p+q}M''_i \delta t_i=
		\sum_{i=1}^{p}M_i \delta t_i + \sum_{i=p+1}^{q}M'_{i-p} \delta t'_{i-p} \\
		      & =U(P,f)+U(Q,f)
	\end{align*}
	Repeating the same argument for lower sums,
	\[ L(P,f)+L(Q,f)= \sum_{i=1}^{p}m_i \delta t_i + \sum_{i=1}^{q}m'_i \delta t'_i   \]
	where $m_i$ and $t_i$ correspond to P, while where $m'_i$ and $t'_i$ correspond to Q.
	Taking $S:= P \cup Q$ so that $S \in \mathbb{P}([a,b]) $,\\
	giving S=$\{a<t_1<t_2<...<c<t'_1<t'_2<...<b\}$

	where $t_i \in P$ and $t'_i \in Q$, so that,\\
	\begin{align*}
		L(S,f)&= \sum_{i=1}^{p+q}m''_i \delta t_i=
		\sum_{i=1}^{p}m_i \delta t_i + \sum_{i=p+1}^{q}m'_{i-p} \delta t'_{i-p} \\
		      & =L(P,f)+L(Q,f)
	\end{align*}
	Hence,
	\begin{align*}
		U(S,f) - L(S,f) &= (U(P,f)+U(Q,f)) - (L(P,f)+L(Q,f))\\
				&= U(P,f)-L(P,f) + U(Q,f)-L(Q,f)\\
				&< \frac{\epsilon}{2}+\frac{\epsilon}{2}= \epsilon
	\end{align*}
\end{proof}
\newpage

\section*{Question 2}
Suppose $P \in \mathbb{P}([a,b])$ such that $U(P,f)=L(P,f)$.\\
Prove that $f$ is a constant function.
\begin{proof}
	As $U(P,f)=L(P,f)$,
	\begin{eqnarray*}
		\sum_{i=1}^{p}M_i \delta t_i = \sum_{i=1}^{p}m_i \delta t_i
		\implies \sum_{i=1}^{p}(M_i-m_i) \delta t_i=0
	\end{eqnarray*}
	But, as each $\delta_i>0$, it must be that each $M_i-m_i=0$.\\
	Hence, $f$ is constant in every $\Delta t_i= [t_{i-1},t_i]$.\\
	So, suppose(if possible) f is not constant over [a,b]  ,\\
	Then, there must be some $\alpha \in \mathbb{N}$ and $\Delta t_k,\Delta t_{k+\alpha}$
	such that $f$ takes distinct values in them.\\
	Then, as $f$ is constant on them, $f(t_k)\neq f(t_{k+\alpha})$\\
	But, $f$ is constant on $\Delta t_k=[t_{k-1},t_k] \text{ and } \Delta t_{k+1}=[t_k,t_{k+1}]$

	and as, $t_k$, is in both, $f$ attains same value on both.\\

	Now, $\Delta t_{k+1} \text{ and } \Delta t_{k+2}$ share $t_{k+1}$ thus fixing
	the value of f to be the same over both of them. And, this is the same
	value as that on $\Delta t_k$, i.e. $f(t_k)$.

	Repeating the above argument $\alpha-2$ more times, the value on  $\Delta t_{k+\alpha}$
	also becomes $f(t_k)$, i.e. $f(t_k)=f(t_{k+\alpha})$\\
	Hence, our supposition was incorrect, and $f$ is constant over [a,b].
\end{proof}
\newpage

\section*{Question 3}
$a_n > 0$ need to show that $ \text{ lim sup} \frac{a_{n+1}}{a_n} \geq \text{ lim sup}(a_n)^{1/n} $
\begin{proof}
	Case 1: \text{lim sup } $ \frac{a_{n+1}}{a_n}=\infty $\\
	As \text{lim sup }$(a_n)^ \frac{1}{n} \leq \infty = \text{lim sup }\frac{a_{n+1}}{a_n}$,done\\

	Case 2: \text{lim sup } $ \frac{a_{n+1}}{a_n}= -\infty $\\
	\[ \text{lim sup }  \frac{a_{n+1}}{a_n}= -\infty \implies \lim_{n \to \infty} \frac{a_{n+1}}{a_n} = -\infty\]
	But, as all $a_n$ are positive, so is their raito, and hence it cant be unbounded below. \\

	Case 3: \text{lim sup } $ \frac{a_{n+1}}{a_n}= a \in \mathbb{R} $\\
	So, $ \forall \epsilon > 0,  \exists M \in \mathbb{N}: n > M \implies \frac{a_{n+1}}{a_n} < a+\epsilon$.\\
	Fix an M. So, as $a \geq 0 \implies (a+\epsilon)>0 $,  for any $n>M$,
	\[ a_n<(a+\epsilon) a_{n-1}<(a+\epsilon)^2 a_{n-2}<...<(a+\epsilon)^{n-M} a_M \]
	Now, as $\frac{a_M}{a^M}$ is a constant, it's n-th root goes to 1 i.e.
	\[   	\exists K \in \mathbb{N}: n \geq K \implies  (\frac{a_M}{a^M})^{ \frac{1}{n} } <1+\epsilon\]
	Thus, by the previous inequality,
	\[ (a_n)^{ \frac{1}{n} } < (a+\epsilon)^{1- \frac{M}{n} }(a_M) ^{ \frac{1}{n} }
		<(a+ \epsilon) (\frac{a_M}{(a+\epsilon)^M})^{ \frac{1}{n} }
	\]
	\[\implies (a_n)^\frac{1}{n}<(a+ \epsilon) (\frac{a_M}{a^M})^{ \frac{1}{n} } < (a+\epsilon)(1+\epsilon)=a+(a+1)\epsilon + \epsilon^2 \]
	Thus,
	\[\text{lim sup }(a_n)^ \frac{1}{n} \leq a+(a+1) \epsilon + \epsilon^2<a+(a+1)(1+\epsilon)\epsilon, \]
	but as this holds for every $\epsilon>0$,
	\[ \text{lim sup }(a_n)^ \frac{1}{n} \leq a= \text{lim sup } \frac{a_{n+1}}{a_n}  \]
\end{proof}
\newpage


\section*{Question 4}
Determine whether $x(1+ \frac{1}{n} )$ converges uniformly on $\mathbb{R}$.
\begin{proof}
	To show pointwise convergance,
	\[ \lim_{n \to \infty} f_n = \lim_{n \to \infty} \big( x + \frac{x}{n} \big) = x \]
	To show that it converges non uniformly,\\
	need an $\epsilon$ for which every $\delta$ fails for some $x \in \mathbb{R}$
	\[ \exists \epsilon : \forall \delta, \exists x \text{ such that }
	\Big( \exists n,m> \delta \text{ with } |f_n(x) - f_m(x)| \geq \epsilon \Big) \]
	Take $\epsilon = 0.5$, and fix any $\delta>0$.

	Now, take $n=\delta+1$ and $m=\delta+2$.
	Take $x= \frac{1}{(\frac{1}{n} - \frac{1}{m})}$\\
	So,
	\begin{align*}
		|f_n(x) - f_m(x)|&=|\Big(x(1+ \frac{1}{n} )-x(1+ \frac{1}{m}) \Big)|\\
				 &=|x\Big((1+ \frac{1}{n} )-(1+ \frac{1}{m} )\Big)|\\
				 &=|\frac{1}{(\frac{1}{n} - \frac{1}{m})}
				 \big(\frac{1}{n} -\frac{1}{m} \big)|=1>0.5=\epsilon\\
	\end{align*}
\end{proof}
\newpage




\end{document}

